extract/Main.hs
@@ -23,12 +23,12 @@ w82c = toEnum . fromIntegral
 w82s :: [Word8] -> String
 w82s = Prelude.map w82c
 
-printPS :: Rep -> CRep -> BScrep -> IO String
-printPS h h' bs =
-    let (bs', mres) = unconsBS h h' bs in
-    case mres of
-        Nothing -> return []
-        Just c  -> (w82c c:) <$> printPS h h' bs'
+-- printPS :: Rep -> CRep -> BScrep -> IO String
+-- printPS h h' bs =
+--     let (bs', mres) = unconsBS h h' bs in
+--     case mres of
+--         Nothing -> return []
+--         Just c  -> (w82c c:) <$> printPS h h' bs'
 
 printPS0 :: PS0 -> IO String
 printPS0 bs =
@@ -45,27 +45,27 @@ printPS1 bs =
 
 main :: IO ()
 main = do
-    putStrLn "ByteString list..."
+    -- putStrLn "ByteString list..."
 
-    let h0 = emptyHeap
-    let b0 = emptyBS any' h0
-    putStrLn . ("b0 = " ++) =<< printPS any' h0 b0
-    let b1 = consBS any' h0 b0 (c2w8 'a')
-    putStrLn . ("b1 = " ++) =<< printPS any' h0 b1
-    let b2 = consBS any' h0 b1 (c2w8 'b')
-    putStrLn . ("b2 = " ++) =<< printPS any' h0 b2
-    let b3 = consBS any' h0 b2 (c2w8 'c')
-    putStrLn . ("b3 = " ++) =<< printPS any' h0 b3
-    let (b4, mres1) = unconsBS any' h0 b3
-    putStrLn . ("b4 = " ++) =<< printPS any' h0 b4
-    print mres1
-    let (b5, mres2) = unconsBS any' h0 b4
-    putStrLn . ("b5 = " ++) =<< printPS any' h0 b5
-    print mres2
+    -- let h0 = emptyHeap
+    -- let b0 = emptyBS any' h0
+    -- putStrLn . ("b0 = " ++) =<< printPS any' h0 b0
+    -- let b1 = consBS any' h0 b0 (c2w8 'a')
+    -- putStrLn . ("b1 = " ++) =<< printPS any' h0 b1
+    -- let b2 = consBS any' h0 b1 (c2w8 'b')
+    -- putStrLn . ("b2 = " ++) =<< printPS any' h0 b2
+    -- let b3 = consBS any' h0 b2 (c2w8 'c')
+    -- putStrLn . ("b3 = " ++) =<< printPS any' h0 b3
+    -- let (b4, mres1) = unconsBS any' h0 b3
+    -- putStrLn . ("b4 = " ++) =<< printPS any' h0 b4
+    -- print mres1
+    -- let (b5, mres2) = unconsBS any' h0 b4
+    -- putStrLn . ("b5 = " ++) =<< printPS any' h0 b5
+    -- print mres2
 
-    -- b3 has the final heap state
-    let b6 = appendBS any' h0 b3 b2
-    putStrLn . ("bs6 = " ++) =<< printPS any' h0 b6
+    -- -- b3 has the final heap state
+    -- let b6 = appendBS any' h0 b3 b2
+    -- putStrLn . ("bs6 = " ++) =<< printPS any' h0 b6
 
     putStrLn "ByteString heap..."
 
@@ -86,9 +86,6 @@ main = do
 
     let bs6 = ghcAppendDSL' bs3 bs2
     putStrLn . ("bs6 = " ++) =<< printPS0 bs6
-
-    let bs6'' = ghcAppendDSL'' bs3 bs2
-    putStrLn . ("bs6'' = " ++) =<< printPS0 bs6''
 
     putStrLn "ByteString via Internal..."
 
@@ -115,21 +112,3 @@ main = do
             putStrLn . ("s6 = " ++) =<< printPS1 s6
   where
     any' = unsafeCoerce ()
-
-ghcAppendDSL'' :: PS0 -> PS0 -> PS0
-ghcAppendDSL'' p p0 = unsafePerformIO $
-  if 0 < psLength0 p
-  then
-    if 0 < psLength0 p0
-    then do
-      cod <- mallocBytes ((+) (psLength0 p) (psLength0 p0))
-      copyBytes cod (plusPtr (unsafeCoerce (psBuffer0 p)) (psOffset0 p))
-                (psLength0 p)
-      copyBytes (plusPtr cod (psLength0 p))
-                (plusPtr (unsafeCoerce (psBuffer0 p0)) (psOffset0 p0))
-                (psLength0 p0)
-      return $ MakePS0 (unsafeCoerce cod)
-                       ((+) (psLength0 p) (psLength0 p0)) 0
-                       ((+) (psLength0 p) (psLength0 p0))
-    else return p
-  else return p0
