src/Heap.v
@@ -65,44 +65,52 @@ Definition HeapSpec := Def ADT {
               Else bytes r |}, naddr),
 
   (* Peeking an uninitialized address allows any value to be returned. *)
-  Def Method1 peekS (r : rep) (addr : Ptr Word) : rep * Word :=
+  Def Method2 peekS (r : rep) (addr : Ptr Word) (off : Size) : rep * Word :=
+    let addr' := plusPtr addr off in
     p <- { p : Word
-         | M.MapsTo addr p (bytes r) \/ (~ M.In addr (bytes r) /\ p = Zero) };
+         | M.MapsTo addr' p (bytes r)
+             \/ (~ M.In addr' (bytes r) /\ p = Zero) };
     ret (r, p),
 
-  Def Method2 pokeS (r : rep) (addr : Ptr Word) (w : Word) : rep :=
+  Def Method3 pokeS (r : rep) (addr : Ptr Word) (off : Size) (w : Word) : rep :=
     ret {| resvs := resvs r
-         ; bytes := M.add addr w (bytes r) |},
+         ; bytes := M.add (plusPtr addr off) w (bytes r) |},
 
   (* Data may only be copied from one allocated block to another (or within
      the same block), and the region must fit within both source and
      destination. Otherwise, the operation is a no-op. *)
-  Def Method3 memcpyS (r : rep)
-      (addr1 : Ptr Word) (addr2 : Ptr Word) (len : Size) : rep :=
+  Def Method5 memcpyS (r : rep) (addr1 : Ptr Word) (off1 : Size)
+                      (addr2 : Ptr Word) (off2 : Size) (len : Size) : rep :=
     ret {| resvs := resvs r
-         ; bytes := copy_bytes addr1 addr2 len (bytes r) |},
+         ; bytes := copy_bytes (A:=Word) (plusPtr addr1 off1)
+                               (plusPtr addr2 off2) len (bytes r) |},
 
   (* Any attempt to memset bytes outside of an allocated block is a no-op. *)
-  Def Method3 memsetS (r : rep) (addr : Ptr Word) (len : Size) (w : Word) : rep :=
+  Def Method4 memsetS (r : rep) (addr : Ptr Word) (off : Size)
+                      (len : Size) (w : Word) : rep :=
     ret {| resvs := resvs r
-         ; bytes := P.update (bytes r)
-                             (N.peano_rect
-                                (fun _ => M.t Word) (bytes r)
-                                (fun i => M.add (plusPtr addr i)%N w) len) |},
+         ; bytes :=
+             P.update (bytes r)
+                      (N.peano_rect
+                         (fun _ => M.t Word) (bytes r)
+                         (fun i => M.add (plusPtr addr (off + i))%N w) len) |},
 
-  Def Method2 readS (r : rep) (addr : Ptr Word) (len : Size) : rep * (list Word) :=
+  Def Method3 readS (r : rep) (addr : Ptr Word) (off : Size) (len : Size) :
+      rep * (list Word) :=
     xs <- { xs : list Word
           | xs = N.peano_rect
                    (fun _ => list Word) []%list
-                   (fun i xs => match M.find (plusPtr addr i) (bytes r) with
-                                | None   => Zero
-                                | Some w => w
-                                end :: xs) len };
+                   (fun i xs =>
+                      match M.find (plusPtr addr (off + i)) (bytes r) with
+                      | None   => Zero
+                      | Some w => w
+                      end :: xs) len };
     ret (r, xs),
 
-  Def Method2 writeS (r : rep) (addr : Ptr Word) (xs : list Word) : rep :=
+  Def Method3 writeS (r : rep) (addr : Ptr Word) (off : Size) (xs : list Word) :
+      rep :=
     ret {| resvs := resvs r
-         ; bytes := load_into_map addr xs (bytes r) |}
+         ; bytes := load_into_map (plusPtr addr off) xs (bytes r) |}
 
 }%ADTParsing.
 
@@ -129,33 +137,34 @@ Definition realloc (r : Rep HeapSpec)
   Comp (Rep HeapSpec * Ptr Word) :=
   Eval simpl in callMeth HeapSpec reallocS r addr len.
 
-Definition peek (r : Rep HeapSpec) (addr : Ptr Word) :
+Definition peek (r : Rep HeapSpec) (addr : Ptr Word) (off : Size) :
   Comp (Rep HeapSpec * Word) :=
-  Eval simpl in callMeth HeapSpec peekS r addr.
+  Eval simpl in callMeth HeapSpec peekS r addr off.
 
-Definition poke (r : Rep HeapSpec) (addr : Ptr Word) (w : Word) :
+Definition poke (r : Rep HeapSpec) (addr : Ptr Word) (off : Size) (w : Word) :
   Comp (Rep HeapSpec) :=
-  Eval simpl in callMeth HeapSpec pokeS r addr w.
+  Eval simpl in callMeth HeapSpec pokeS r addr off w.
 
 Definition memcpy (r : Rep HeapSpec)
-           (addr : Ptr Word) (addr2 : Ptr Word) (len : Size) :
+           (addr1 : Ptr Word) (off1 : Size)
+           (addr2 : Ptr Word) (off2 : Size) (len : Size) :
   Comp (Rep HeapSpec) :=
-  Eval simpl in callMeth HeapSpec memcpyS r addr addr2 len.
+  Eval simpl in callMeth HeapSpec memcpyS r addr1 off1 addr2 off2 len.
 
 Definition memset (r : Rep HeapSpec)
-           (addr : Ptr Word) (len : Ptr Word) (w : Word) :
+           (addr : Ptr Word) (off : Size) (len : Ptr Word) (w : Word) :
   Comp (Rep HeapSpec) :=
-  Eval simpl in callMeth HeapSpec memsetS r addr len w.
+  Eval simpl in callMeth HeapSpec memsetS r addr off len w.
 
 Definition read (r : Rep HeapSpec)
-           (addr : Ptr Word) (len : Ptr Word) :
+           (addr : Ptr Word) (off : Size) (len : Ptr Word) :
   Comp (Rep HeapSpec * list Word) :=
-  Eval simpl in callMeth HeapSpec readS r addr len.
+  Eval simpl in callMeth HeapSpec readS r addr off len.
 
 Definition write (r : Rep HeapSpec)
-           (addr : Ptr Word) (xs : list Word) :
+           (addr : Ptr Word) (off : Size) (xs : list Word) :
   Comp (Rep HeapSpec) :=
-  Eval simpl in callMeth HeapSpec writeS r addr xs.
+  Eval simpl in callMeth HeapSpec writeS r addr off xs.
 
 (**
  ** Theorems related to the Heap specification.
@@ -324,7 +333,7 @@ Lemma refine_realloc : forall (addr : Ptr Word) len r,
     -> sz <= ` len
     -> refine (realloc r addr len)
               (`(r, addr') <- alloc r len;
-               r <- memcpy r addr addr' sz;
+               r <- memcpy r addr 0 addr' 0 sz;
                r <- free r addr;
                ret (r, addr')).
 Proof.
@@ -376,7 +385,7 @@ Proof.
     repeat simplify_maps.
     right.
     intuition.
-  rewrite N.min_l; trivial.
+  rewrite N.min_l, !plusPtr_zero; trivial.
 Qed.
 
 End Heap.
