extract/fixcode.pl
@@ -16,6 +16,7 @@ import qualified Foreign.Marshal.Utils
 import qualified Foreign.Ptr
 import qualified Foreign.Storable
 import qualified GHC.Real
+import qualified GHC.ForeignPtr
 import qualified Prelude
 import qualified System.IO.Unsafe
 END_IMPORTS
@@ -24,6 +25,35 @@ while (<>) {
     next if /^ghcDenote ::/ .. /^$/;
     next if /^heapCanonical0 ::/ .. /^$/;
     next if /^byteStringHeap0 ::/ .. /^$/;
+    next if /^compare3 ::/ .. /^$/;
+    next if /^within_bool ::/ .. /^$/;
+    next if /^within_bool0 ::/ .. /^$/;
+    next if /^fits_bool ::/ .. /^$/;
+    next if /^fits_bool0 ::/ .. /^$/;
+    next if /^overlaps_bool ::/ .. /^$/;
+    next if /^overlaps_bool0 ::/ .. /^$/;
+    next if /^keep_range ::/ .. /^$/;
+    next if /^keep_range0 ::/ .. /^$/;
+    next if /^drop_range ::/ .. /^$/;
+    next if /^drop_range0 ::/ .. /^$/;
+    next if /^copy_bytes ::/ .. /^$/;
+    next if /^copy_bytes0 ::/ .. /^$/;
+    next if /^load_into_map ::/ .. /^$/;
+    next if /^load_into_map0 ::/ .. /^$/;
+    next if /^heapSpec ::/ .. /^$/;
+    next if /^heapSpec0 ::/ .. /^$/;
+    next if /^heapCanonical ::/ .. /^$/;
+    next if /^byteStringHeap ::/ .. /^$/;
+    next if /^byteStringCanonical ::/ .. /^$/;
+    next if /^buffer_to_list ::/ .. /^$/;
+    next if /^buffer_to_list0 ::/ .. /^$/;
+
+    next if /^emptyBS ::/ .. /^$/;
+    next if /^packBS ::/ .. /^$/;
+    next if /^unpackBS ::/ .. /^$/;
+    next if /^consBS ::/ .. /^$/;
+    next if /^unconsBS ::/ .. /^$/;
+    next if /^appendBS ::/ .. /^$/;
 
     next if /^emptyDSL ::/ .. /^$/;
     next if /^ghcEmptyDSL ::/ .. /^$/;
